VeilTest/Regression/SimulateDeadlock.lean
@@ -26,7 +26,7 @@ error: ❌ Violation: deadlock
 Seed: 1
 -/
 #guard_msgs in
-#simulate interpreted {} {} (seed := 1) (maxTraces := 1) (maxSteps := 1)
+#simulate interpreted {} {} (seed := 1) (numTraces := 1) (maxSteps := 1)
 
 end SimulateDeadlock
 
@@ -64,6 +64,6 @@ error: ❌ Violation: deadlock
 Seed: 1
 -/
 #guard_msgs in
-#simulate interpreted {} {} (seed := 1) (maxTraces := 1) (maxSteps := 3)
+#simulate interpreted {} {} (seed := 1) (numTraces := 1) (maxSteps := 3)
 
 end SimulateDeadlockAfterStep
